Equiv between Binary step and denotation
Finished the proof of BinStep.multi_cstep <-> BinRel.ceval

DenotationalSemantics.v
@@ -4,9 +4,64 @@ Require Import PL.Imp3.
 (** Definition of Denotational Semantics as Binary Relation
     (Begin States, Ending States). *)
 
+Inductive semantic (X: Type) :=
+  | Sem (skip_sem: X)
+        (asgn_sem: var -> aexp -> X)
+        (seq_sem: X -> X -> X)
+        (if_sem: bexp -> X -> X -> X)
+        (loop_sem: bexp -> X -> X).
+
+Arguments Sem {X} skip_sem asgn_sem seq_sem if_sem loop_sem.
+
+Definition semantic_skip {X: Type} (S: semantic X) := 
+  match S with
+  | Sem skip_sem _ _ _ _ => skip_sem
+  end.
+
+Definition semantic_asgn {X: Type} (S: semantic X) := 
+  match S with
+  | Sem _ asgn_sem _ _ _ => asgn_sem
+  end.
+
+Definition semantic_seq {X: Type} (S: semantic X) := 
+  match S with
+  | Sem _ _ seq_sem _ _ => seq_sem
+  end.
+
+Definition semantic_if {X: Type} (S: semantic X) := 
+  match S with
+  | Sem _ _ _ if_sem _ => if_sem
+  end.
+
+Definition semantic_loop {X: Type} (S: semantic X) := 
+  match S with
+  | Sem _ _ _ _ loop_sem => loop_sem
+  end.
+
+Fixpoint ceval_by_sem {T: Type} (S: semantic T)
+  (c : com) : T :=
+  match c with
+  | CSkip => semantic_skip S
+  | CAss X E => semantic_asgn S X E
+  | CSeq c1 c2 => semantic_seq S (ceval_by_sem S c1) (ceval_by_sem S c2)
+  | CIf b c1 c2 => semantic_if S b (ceval_by_sem S c1) (ceval_by_sem S c2)
+  | CWhile b c => semantic_loop S b (ceval_by_sem S c)
+  end.
+
 Module BinRel.
 
 Import Relation_Operators.
+
+Definition skip_sem: state -> state -> Prop := id.
+
+Definition asgn_sem (X: var) (E: aexp): state -> state -> Prop :=
+  fun st1 st2 =>
+    st2 X = aeval E st1 /\
+    forall Y, X <> Y -> st1 Y = st2 Y.
+
+Definition seq_sem (c1 c2: state -> state -> Prop)
+  : state -> state -> Prop
+:= concat c1 c2.
 
 Definition if_sem
   (b: bexp)
@@ -35,17 +90,41 @@ Definition loop_sem (b: bexp) (loop_body: state -> state -> Prop):
   state -> state -> Prop :=
   omega_union (iter_loop_body b loop_body).
 
-Fixpoint ceval (c: com): state -> state -> Prop :=
-  match c with
-  | CSkip => id
-  | CAss X E =>
-      fun st1 st2 =>
-        st2 X = aeval E st1 /\
-        forall Y, X <> Y -> st1 Y = st2 Y
-  | CSeq c1 c2 => concat (ceval c1) (ceval c2)
-  | CIf b c1 c2 => if_sem b (ceval c1) (ceval c2)
-  | CWhile b c => loop_sem b (ceval c)
-  end.
+Definition sem := Sem skip_sem asgn_sem seq_sem if_sem loop_sem.
+
+Definition ceval := ceval_by_sem sem.
+
+Lemma ceval_CSkip: ceval CSkip = id.
+Proof. intros. simpl. reflexivity. Qed.
+
+Lemma ceval_CAss: forall X E,
+  ceval (CAss X E) =
+    fun st1 st2 =>
+      st2 X = aeval E st1 /\
+        forall Y, X <> Y -> st1 Y = st2 Y.
+Proof. intros. simpl. reflexivity. Qed.
+
+Lemma ceval_CSeq: forall c1 c2,
+  ceval (c1 ;; c2) = concat (ceval c1) (ceval c2).
+Proof. intros. simpl. reflexivity. Qed.
+
+Lemma ceval_CIf: forall b c1 c2,
+  ceval (CIf b c1 c2) = if_sem b (ceval c1) (ceval c2).
+Proof. intros. simpl. reflexivity. Qed.
+
+Lemma ceval_CWhile: forall b c,
+  ceval (While b Do c EndWhile) = loop_sem b (ceval c).
+Proof. intros. simpl. reflexivity. Qed.
+
+Theorem loop_unrolling : forall b c st1 st2,
+  ceval (While b Do c EndWhile) st1 st2 <->
+  ceval (If b Then (c ;; While b Do c EndWhile) Else Skip EndIf) st1 st2.
+Proof.
+  intros.
+  rewrite ceval_CIf, ceval_CSeq, ceval_CSkip.
+  rewrite ceval_CWhile.
+  apply loop_sem_unrolling.
+Qed.
 
 End BinRel.
 
@@ -111,14 +190,91 @@ Definition loop_sem (b: bexp) (loop_body: state -> Z -> state -> Prop)
 :=
   omega_union_sem (iter_loop_body b loop_body).
 
-Fixpoint ceval (c: com): state -> Z -> state -> Prop :=
-  match c with
-  | CSkip => skip_sem
-  | CAss X E => asgn_sem X E
-  | CSeq c1 c2 => seq_sem (ceval c1) (ceval c2)
-  | CIf b c1 c2 => if_sem b (ceval c1) (ceval c2)
-  | CWhile b c => loop_sem b (ceval c)
-  end.
+Definition sem := Sem skip_sem asgn_sem seq_sem if_sem loop_sem.
+
+Definition ceval := ceval_by_sem sem.
+
+Lemma ceval_CSkip: ceval CSkip = skip_sem.
+Proof. intros. simpl. reflexivity. Qed.
+
+Lemma ceval_CAss: forall X E,
+  ceval (CAss X E) =
+    fun st1 z st2 =>
+      st2 X = aeval E st1 /\
+        forall Y, X <> Y -> st1 Y = st2 Y /\
+        z = 1.
+Proof. intros. simpl. reflexivity. Qed.
+
+Lemma ceval_CSeq: forall c1 c2,
+  ceval (c1 ;; c2) = seq_sem (ceval c1) (ceval c2).
+Proof. intros. simpl. reflexivity. Qed.
+
+Lemma ceval_CIf: forall b c1 c2,
+  ceval (CIf b c1 c2) = if_sem b (ceval c1) (ceval c2).
+Proof. intros. simpl. reflexivity. Qed.
+
+Lemma ceval_CWhile: forall b c,
+  ceval (While b Do c EndWhile) = loop_sem b (ceval c).
+Proof. intros. simpl. reflexivity. Qed.
+
+Lemma loop_sem_unrolling: forall b (R: state -> Z -> state -> Prop) st1 z st2,
+  loop_sem b R st1 z st2 <-> 
+  if_sem b (seq_sem R (loop_sem b R)) skip_sem st1 z st2.
+Proof.
+  split; intros.
+  + unfold loop_sem, omega_union_sem in H.
+    destruct H as [n ?].
+    destruct n.
+    - simpl in H.
+      unfold if_sem, seq_sem.
+      right; simpl.
+      unfold skip_sem.
+      exists z, 0, st2; split; [exact H | split; [tauto | lia]].
+    - simpl in H.
+      unfold if_sem, seq_sem.
+      left.
+      unfold seq_sem in H.
+      destruct H as [z1 [z2 [st1' [[Hst [Hb Hz1]] H]]]].
+      destruct H as [[z3 [z4 [st3 [Hc [Hiter Hz3]]]]] Hz2].
+      subst z1 z2 z st1'.
+      exists 1, (z3 + z4), st1; split; [unfold test_sem; tauto | split; [| lia]].
+      exists z3, z4, st3; split; [tauto | split; [| lia]].
+      unfold loop_sem, omega_union_sem.
+      exists n.
+      exact Hiter.
+  + unfold if_sem, seq_sem in H.
+    unfold loop_sem, omega_union_sem.
+    destruct H.
+    2: {
+      exists O.
+      simpl.
+      unfold skip_sem in H.
+      destruct H as [z1 [z2 [st2' [[Hst [Hb Hz1]] [[Hst2 Hz2] Hz]]]]].
+      subst z1 z2 z st2' st2.
+      unfold test_sem.
+      split; [tauto | split; [tauto | lia]].
+    }
+    destruct H as [z1 [z2 [st1' [[Hst [Hb Hz1]] H]]]].
+    destruct H as [[z3 [z4 [st3 [Hc [Hiter Hz3]]]]] Hz2].
+    subst z1 z2 z st1'.
+    unfold loop_sem, omega_union_sem in Hiter.
+    destruct Hiter as [n Hiter].
+    exists (S n).
+    simpl.
+    unfold seq_sem.
+    exists 1, (z3 + z4), st1; split; [unfold test_sem; tauto | split; [| tauto]].
+    exists z3, z4, st3; tauto.
+Qed.
+
+Theorem loop_unrolling : forall b c z st1 st2,
+  ceval (While b Do c EndWhile) st1 z st2 <->
+  ceval (If b Then (c ;; While b Do c EndWhile) Else Skip EndIf) st1 z st2.
+Proof.
+  intros.
+  rewrite ceval_CIf, ceval_CSeq, ceval_CSkip.
+  rewrite ceval_CWhile.
+  apply loop_sem_unrolling.
+Qed.
 
 End StepCnt.
 
@@ -186,13 +342,92 @@ Definition loop_sem (b: bexp) (loop_body: state -> list state -> state -> Prop)
 :=
   omega_union_sem (iter_loop_body b loop_body).
 
-Fixpoint ceval (c: com): state -> list state -> state -> Prop :=
-  match c with
-  | CSkip => skip_sem
-  | CAss X E => asgn_sem X E
-  | CSeq c1 c2 => seq_sem (ceval c1) (ceval c2)
-  | CIf b c1 c2 => if_sem b (ceval c1) (ceval c2)
-  | CWhile b c => loop_sem b (ceval c)
-  end.
+Definition sem := Sem skip_sem asgn_sem seq_sem if_sem loop_sem.
+
+Definition ceval := ceval_by_sem sem.
+
+Lemma ceval_CSkip: ceval CSkip = skip_sem.
+Proof. intros. simpl. reflexivity. Qed.
+
+Lemma ceval_CAss: forall X E,
+  ceval (CAss X E) =
+    fun st1 l st2 =>
+      st2 X = aeval E st1 /\
+        forall Y, X <> Y -> st1 Y = st2 Y /\
+        l = st2 :: nil.
+Proof. intros. simpl. reflexivity. Qed.
+
+Lemma ceval_CSeq: forall c1 c2,
+  ceval (c1 ;; c2) = seq_sem (ceval c1) (ceval c2).
+Proof. intros. simpl. reflexivity. Qed.
+
+Lemma ceval_CIf: forall b c1 c2,
+  ceval (CIf b c1 c2) = if_sem b (ceval c1) (ceval c2).
+Proof. intros. simpl. reflexivity. Qed.
+
+Lemma ceval_CWhile: forall b c,
+  ceval (While b Do c EndWhile) = loop_sem b (ceval c).
+Proof. intros. simpl. reflexivity. Qed.
+
+Lemma loop_sem_unrolling: forall b (R: state -> list state -> state -> Prop) st1 l st2,
+  loop_sem b R st1 l st2 <-> 
+  if_sem b (seq_sem R (loop_sem b R)) skip_sem st1 l st2.
+Proof.
+  split; intros.
+  + unfold loop_sem, omega_union_sem in H.
+    destruct H as [n ?].
+    destruct n.
+    - simpl in H.
+      unfold if_sem, seq_sem.
+      right; simpl.
+      unfold skip_sem.
+      exists l, nil, st2; split; [exact H | split; [tauto | apply app_nil_end]].
+    - simpl in H.
+      unfold if_sem, seq_sem.
+      left.
+      unfold seq_sem in H.
+      destruct H as [l1 [l2 [st1' [[Hst [Hb Hl1]] H]]]].
+      destruct H as [[l3 [l4 [st3 [Hc [Hiter Hl3]]]]] Hl2].
+      subst l1 l2 l st1'.
+      exists (st1 :: nil), (l3 ++ l4), st1; split;
+        [unfold test_sem; tauto | split; [| reflexivity]].
+      exists l3, l4, st3; split; [tauto | split; [| reflexivity]].
+      unfold loop_sem, omega_union_sem.
+      exists n.
+      exact Hiter.
+  + unfold if_sem, seq_sem in H.
+    unfold loop_sem, omega_union_sem.
+    destruct H.
+    2: {
+      exists O.
+      simpl.
+      unfold skip_sem in H.
+      destruct H as [l1 [l2 [st2' [[Hst [Hb Hl1]] [[Hst2 Hl2] Hl]]]]].
+      subst l1 l2 l st2' st2.
+      unfold test_sem.
+      split; [tauto | split; [reflexivity | tauto]].
+    }
+    destruct H as [l1 [l2 [st1' [[Hst [Hb Hl1]] H]]]].
+    destruct H as [[l3 [l4 [st3 [Hc [Hiter Hl3]]]]] Hl2].
+    subst l1 l2 l st1'.
+    unfold loop_sem, omega_union_sem in Hiter.
+    destruct Hiter as [n Hiter].
+    exists (S n).
+    simpl.
+    unfold seq_sem.
+    exists (st1 :: nil), (l3 ++ l4), st1;
+      split; [unfold test_sem; tauto | split; [| tauto]].
+    exists l3, l4, st3; tauto.
+Qed.
+
+Theorem loop_unrolling : forall b c z st1 st2,
+  ceval (While b Do c EndWhile) st1 z st2 <->
+  ceval (If b Then (c ;; While b Do c EndWhile) Else Skip EndIf) st1 z st2.
+Proof.
+  intros.
+  rewrite ceval_CIf, ceval_CSeq, ceval_CSkip.
+  rewrite ceval_CWhile.
+  apply loop_sem_unrolling.
+Qed.
 
 End Trace.
