DenotationalSemEquiv.v
@@ -1,0 +1,409 @@
+Require Import Coq.Lists.List.
+Require Import PL.Imp3.
+Require Import PL.DenotationalSemantics.
+
+(** In this task, you should first prove a general theorem which can be used to
+    prove an equivalence between two recursively defined semantics, and another
+    general theorem which can be used to prove an equivalence between a
+    recursively defined program semantics and a small step semantics.
+
+    Then, you need to prove the equivalence among three denotational program
+    semantics and a small step semantics. *)
+
+(* Some try before the general theorem *)
+
+Definition Bin_Ter_sem_equiv {M: Type}
+                             (X : state -> state -> Prop)
+                             (Y : state -> M -> state -> Prop) : Prop :=
+  forall st1 st2, X st1 st2 <-> (exists z, Y st1 z st2).
+
+Definition sem_equiv {X Y: Type}
+                     (ceval_X: com -> X)
+                     (ceval_Y: com -> Y)
+                     (RXY: X -> Y -> Prop) : Prop :=
+  forall c, RXY (ceval_X c) (ceval_Y c).
+
+Definition Bin_Ter_skip_sem_equiv {M: Type}
+  (SBin : semantic (state -> state -> Prop))
+  (STer : semantic (state -> M -> state -> Prop)) : Prop :=
+  Bin_Ter_sem_equiv (semantic_skip SBin) (semantic_skip STer).
+
+Definition Bin_Ter_asgn_sem_equiv {M: Type}
+  (SBin : semantic (state -> state -> Prop))
+  (STer : semantic (state -> M -> state -> Prop)) : Prop :=
+  forall X E,
+  Bin_Ter_sem_equiv (semantic_asgn SBin X E) (semantic_asgn STer X E).
+
+Definition Bin_Ter_seq_sem_equiv {M: Type}
+  (SBin : semantic (state -> state -> Prop))
+  (STer : semantic (state -> M -> state -> Prop)) : Prop :=
+  forall c1 c2,
+  Bin_Ter_sem_equiv (ceval_by_sem SBin c1) (ceval_by_sem STer c1) ->
+  Bin_Ter_sem_equiv (ceval_by_sem SBin c2) (ceval_by_sem STer c2) ->
+  Bin_Ter_sem_equiv
+    (semantic_seq SBin (ceval_by_sem SBin c1) (ceval_by_sem SBin c2))
+    (semantic_seq STer (ceval_by_sem STer c1) (ceval_by_sem STer c2)).
+
+Definition Bin_Ter_if_sem_equiv {M: Type}
+  (SBin : semantic (state -> state -> Prop))
+  (STer : semantic (state -> M -> state -> Prop)) : Prop :=
+  forall b c1 c2,
+  Bin_Ter_sem_equiv (ceval_by_sem SBin c1) (ceval_by_sem STer c1) ->
+  Bin_Ter_sem_equiv (ceval_by_sem SBin c2) (ceval_by_sem STer c2) ->
+  Bin_Ter_sem_equiv
+    (semantic_if SBin b (ceval_by_sem SBin c1) (ceval_by_sem SBin c2))
+    (semantic_if STer b (ceval_by_sem STer c1) (ceval_by_sem STer c2)).
+
+Definition Bin_Ter_loop_sem_equiv {M: Type}
+  (SBin : semantic (state -> state -> Prop))
+  (STer : semantic (state -> M -> state -> Prop)) : Prop :=
+  forall b c,
+  Bin_Ter_sem_equiv (ceval_by_sem SBin c) (ceval_by_sem STer c) ->
+  Bin_Ter_sem_equiv
+    (semantic_loop SBin b (ceval_by_sem SBin c))
+    (semantic_loop STer b (ceval_by_sem STer c)).
+
+Theorem Bin_Step_skip_sem_equiv:
+  Bin_Ter_skip_sem_equiv (BinRel.sem) (StepCnt.sem).
+Proof.
+  unfold Bin_Ter_skip_sem_equiv. simpl.
+  unfold Bin_Ter_sem_equiv. intros.
+  unfold BinRel.skip_sem, StepCnt.skip_sem.
+  split.
+  - intros. exists 0. tauto.
+  - intros [z [H1 H2]].
+    tauto.
+Qed.
+
+Theorem Bin_Step_asgn_sem_equiv:
+  Bin_Ter_asgn_sem_equiv (BinRel.sem) (StepCnt.sem).
+Proof.
+  unfold Bin_Ter_asgn_sem_equiv. simpl.
+  unfold Bin_Ter_sem_equiv. intros.
+  unfold BinRel.asgn_sem,StepCnt.asgn_sem.
+  split.
+  - intros [H1 H2]. exists 1.
+    split. { tauto. }
+    intros. split. { apply (H2 _ H). }
+    tauto.
+  - intros [z [H1 H2]].
+    split. { tauto. }
+    intros. {apply (H2 _ H). }
+Qed.
+
+Theorem Bin_Step_seq_sem_equiv:
+  Bin_Ter_seq_sem_equiv (BinRel.sem) (StepCnt.sem).
+Proof.
+  unfold Bin_Ter_seq_sem_equiv. simpl.
+  unfold Bin_Ter_sem_equiv. intros.
+  unfold BinRel.seq_sem, StepCnt.seq_sem, Relation_Operators.concat.
+  split.
+  - intros [st3 [H1 H2]].
+    destruct (H st1 st3) as [H1' H1''].
+    destruct (H1' H1) as [z1 HE1].
+    destruct (H0 st3 st2) as [H2' H2''].
+    destruct (H2' H2) as [z2 HE2].
+    exists (z1 + z2), z1, z2, st3.
+    tauto.
+  - intros [z [z1 [z2 [st3 [H1 [H2 Hz]]]]]].
+    destruct (H st1 st3) as [H1' H1''].
+    destruct (H0 st3 st2) as [H2' H2''].
+    exists st3.
+    split.
+    + apply H1''.
+      exists z1. apply H1.
+    + apply H2''.
+      exists z2. apply H2.
+Qed.
+
+Theorem Bin_Step_if_sem_equiv:
+  Bin_Ter_if_sem_equiv (BinRel.sem) (StepCnt.sem).
+Proof.
+  unfold Bin_Ter_if_sem_equiv. simpl.
+  unfold Bin_Ter_sem_equiv. intros.
+  unfold semantic_if, BinRel.if_sem, StepCnt.if_sem.
+  unfold Relation_Operators.union,
+         Relation_Operators.concat,
+         Relation_Operators.test_rel.
+  split; intros.
+  + destruct H1.
+    - destruct H1 as [st3 [[Hst Hb] H1]]. subst st3.
+      destruct (H st1 st2) as [H' H''].
+      destruct (H' H1) as [zc Hc].
+      exists (zc + 1). left.
+      exists 1, zc, st1.
+      repeat split.
+      * unfold StepCnt.test_sem; tauto.
+      * exact Hc.
+      * lia.
+    - destruct H1 as [st3 [[Hst Hb] H1]]. subst st3.
+      destruct (H0 st1 st2) as [H' H''].
+      destruct (H' H1) as [zc Hc].
+      exists (zc + 1). right.
+      exists 1, zc, st1.
+      repeat split.
+      * unfold StepCnt.test_sem; tauto.
+      * exact Hc.
+      * lia.
+  + destruct H1 as [z H1];
+      destruct H1;
+      unfold StepCnt.seq_sem in H1;
+      destruct H1 as [z1 [z2 [st3 [[Hst [Hb ?]] [Hc Hz]]]]];
+      subst st3 z1 z.
+    - destruct (H st1 st2) as [H' H''].
+      left. exists st1.
+      repeat split.
+      * exact Hb.
+      * apply H''.
+        exists z2. exact Hc.
+    - destruct (H0 st1 st2) as [H' H''].
+      right. exists st1.
+      repeat split.
+      * exact Hb.
+      * apply H''.
+        exists z2. exact Hc.
+Qed.
+
+Theorem Bin_Step_loop_sem_equiv:
+  Bin_Ter_loop_sem_equiv (BinRel.sem) (StepCnt.sem).
+Proof.
+  unfold Bin_Ter_loop_sem_equiv. simpl.
+  unfold Bin_Ter_sem_equiv. intros.
+  unfold BinRel.loop_sem, Relation_Operators.omega_union.
+  unfold StepCnt.loop_sem, StepCnt.omega_union_sem.
+  split; intros.
+  + destruct H0 as [n H0].
+    revert st1 st2 H0.
+    induction n; intros; simpl in H0.
+    - exists 1, O. simpl.
+      unfold Relation_Operators.test_rel in H0.
+      unfold StepCnt.test_sem.
+      tauto.
+    - unfold Relation_Operators.concat, Relation_Operators.test_rel in H0.
+      destruct H0 as [st1' [[Hst Hb] [st3 [H1 H2]]]]. subst st1'.
+      destruct (IHn _ _ H2) as [zn [n_iter Hn]].
+      destruct (H st1 st3) as [H' H''].
+      destruct (H' H1) as [zc Hc].
+      exists (1 + (zc + zn)), (S n_iter).
+      simpl. unfold StepCnt.seq_sem.
+      exists 1, (zc + zn), st1.
+      repeat split.
+      * exact Hb.
+      * exists zc, zn, st3.
+        repeat split; [exact Hc | exact Hn].
+  + destruct H0 as [z [n H0]].
+    revert z st1 st2 H0.
+    induction n; intros; simpl in H0.
+    - exists O. simpl.
+      unfold StepCnt.test_sem in H0.
+      unfold Relation_Operators.test_rel.
+      tauto.
+    - unfold StepCnt.seq_sem, StepCnt.test_sem in H0.
+      destruct H0 as [z0 [z1 [st1' [[Hst [Hb Ha0]] H0]]]].
+      destruct H0 as [[zc [zn [st3 [Hz' [Hn' Hz2]]]]] Hz1].
+      subst st1' z0 z1 z.
+      destruct (IHn zn st3 st2 Hn') as [n_iter Hn].
+      destruct (H st1 st3) as [H' H''].
+      exists (S n_iter). simpl.
+      unfold Relation_Operators.concat, Relation_Operators.test_rel.
+      exists st1. repeat split. { exact Hb. }
+      exists st3. split.
+      * apply H''. exists zc. exact Hz'.
+      * exact Hn.
+Qed.
+
+Theorem Bin_Trace_skip_sem_equiv:
+  Bin_Ter_skip_sem_equiv (BinRel.sem) (Trace.sem).
+Proof.
+  unfold Bin_Ter_skip_sem_equiv. simpl.
+  unfold Bin_Ter_sem_equiv. intros.
+  unfold BinRel.skip_sem, Trace.skip_sem.
+  split.
+  - intros. exists nil. tauto.
+  - intros [l [H1 H2]].
+    tauto.
+Qed.
+
+Theorem Bin_Trace_asgn_sem_equiv:
+  Bin_Ter_asgn_sem_equiv (BinRel.sem) (Trace.sem).
+Proof.
+  unfold Bin_Ter_asgn_sem_equiv. simpl.
+  unfold Bin_Ter_sem_equiv. intros.
+  unfold BinRel.asgn_sem, Trace.asgn_sem.
+  split.
+  - intros [H1 H2]. exists (st2 :: nil).
+    split. { tauto. }
+    intros. split. { apply (H2 _ H). }
+    tauto.
+  - intros [l [H1 H2]].
+    split. { tauto. }
+    intros. {apply (H2 _ H). }
+Qed.
+
+Theorem Bin_Trace_seq_sem_equiv:
+  Bin_Ter_seq_sem_equiv (BinRel.sem) (Trace.sem).
+Proof.
+  unfold Bin_Ter_seq_sem_equiv. simpl.
+  unfold Bin_Ter_sem_equiv. intros.
+  unfold BinRel.seq_sem, Trace.seq_sem, Relation_Operators.concat.
+  split.
+  - intros [st3 [H1 H2]].
+    destruct (H st1 st3) as [H1' H1''].
+    destruct (H1' H1) as [l1 HE1].
+    destruct (H0 st3 st2) as [H2' H2''].
+    destruct (H2' H2) as [l2 HE2].
+    exists (l1 ++ l2), l1, l2, st3.
+    tauto.
+  - intros [l [l1 [l2 [st3 [H1 [H2 Hl]]]]]].
+    destruct (H st1 st3) as [H1' H1''].
+    destruct (H0 st3 st2) as [H2' H2''].
+    exists st3.
+    split.
+    + apply H1''.
+      exists l1. apply H1.
+    + apply H2''.
+      exists l2. apply H2.
+Qed.
+
+Theorem Bin_Trace_if_sem_equiv:
+  Bin_Ter_if_sem_equiv (BinRel.sem) (Trace.sem).
+Proof.
+  unfold Bin_Ter_if_sem_equiv. simpl.
+  unfold Bin_Ter_sem_equiv. intros.
+  unfold semantic_if, BinRel.if_sem, Trace.if_sem.
+  unfold Relation_Operators.union,
+         Relation_Operators.concat,
+         Relation_Operators.test_rel.
+  split; intros.
+  + destruct H1.
+    - destruct H1 as [st3 [[Hst Hb] H1]]. subst st3.
+      destruct (H st1 st2) as [H' H''].
+      destruct (H' H1) as [lc Hc].
+      exists ((st1 :: nil) ++ lc). left.
+      exists (st1 :: nil), lc, st1.
+      repeat split.
+      * unfold Trace.test_sem; tauto.
+      * exact Hc.
+    - destruct H1 as [st3 [[Hst Hb] H1]]. subst st3.
+      destruct (H0 st1 st2) as [H' H''].
+      destruct (H' H1) as [lc Hc].
+      exists ((st1 :: nil) ++ lc). right.
+      exists (st1 :: nil), lc, st1.
+      repeat split.
+      * unfold Trace.test_sem; tauto.
+      * exact Hc.
+  + destruct H1 as [l H1];
+      destruct H1;
+      unfold Trace.seq_sem in H1;
+      destruct H1 as [l1 [l2 [st3 [[Hst [? Hb]] [Hc Hl]]]]];
+      subst st3 l1 l.
+    - destruct (H st1 st2) as [H' H''].
+      left. exists st1.
+      repeat split.
+      * exact Hb.
+      * apply H''. exists l2. exact Hc.
+    - destruct (H0 st1 st2) as [H' H''].
+      right. exists st1.
+      repeat split.
+      * exact Hb.
+      * apply H''. exists l2. exact Hc.
+Qed.
+
+Theorem Bin_Trace_loop_sem_equiv:
+  Bin_Ter_loop_sem_equiv (BinRel.sem) (Trace.sem).
+Proof.
+  unfold Bin_Ter_loop_sem_equiv. simpl.
+  unfold Bin_Ter_sem_equiv. intros.
+  unfold BinRel.loop_sem, Relation_Operators.omega_union.
+  unfold Trace.loop_sem, Trace.omega_union_sem.
+  split; intros.
+  + destruct H0 as [n H0].
+    revert st1 st2 H0.
+    induction n; intros; simpl in H0.
+    - exists (st1 :: nil), O. simpl.
+      unfold Relation_Operators.test_rel in H0.
+      unfold Trace.test_sem.
+      tauto.
+    - unfold Relation_Operators.concat, Relation_Operators.test_rel in H0.
+      destruct H0 as [st1' [[Hst Hb] [st3 [H1 H2]]]]. subst st1'.
+      destruct (IHn _ _ H2) as [ln [n_iter Hn]].
+      destruct (H st1 st3) as [H' H''].
+      destruct (H' H1) as [lc Hc].
+      exists ((st1 :: nil) ++ (lc ++ ln)), (S n_iter).
+      simpl. unfold Trace.seq_sem.
+      exists (st1 :: nil), (lc ++ ln), st1.
+      repeat split.
+      * exact Hb.
+      * exists lc, ln, st3.
+        repeat split; [exact Hc | exact Hn].
+  + destruct H0 as [l [n H0]].
+    revert l st1 st2 H0.
+    induction n; intros; simpl in H0.
+    - exists O. simpl.
+      unfold Trace.test_sem in H0.
+      unfold Relation_Operators.test_rel.
+      tauto.
+    - unfold Trace.seq_sem, Trace.test_sem in H0.
+      destruct H0 as [l0 [l1 [st1' [[Hst [Ha0 Hb]] H0]]]].
+      destruct H0 as [[lc [ln [st3 [Hl' [Hn' Hl2]]]]] Hl1].
+      subst st1' l0 l1 l.
+      destruct (IHn ln st3 st2 Hn') as [n_iter Hn].
+      destruct (H st1 st3) as [H' H''].
+      exists (S n_iter). simpl.
+      unfold Relation_Operators.concat, Relation_Operators.test_rel.
+      exists st1. repeat split. { exact Hb. }
+      exists st3. split.
+      * apply H''. exists lc. exact Hl'.
+      * exact Hn.
+Qed.
+
+Theorem command_equiv__sem_equiv:
+  forall (M: Type)
+    (SBin : semantic (state -> state -> Prop))
+    (STer : semantic (state -> M -> state -> Prop)),
+  Bin_Ter_skip_sem_equiv SBin STer ->
+  Bin_Ter_asgn_sem_equiv SBin STer ->
+  Bin_Ter_seq_sem_equiv SBin STer ->
+  Bin_Ter_if_sem_equiv SBin STer ->
+  Bin_Ter_loop_sem_equiv SBin STer ->
+  sem_equiv (ceval_by_sem SBin) (ceval_by_sem STer) (Bin_Ter_sem_equiv).
+Proof.
+  unfold Bin_Ter_skip_sem_equiv,
+         Bin_Ter_asgn_sem_equiv,
+         Bin_Ter_seq_sem_equiv,
+         Bin_Ter_if_sem_equiv,
+         Bin_Ter_loop_sem_equiv,
+         sem_equiv,Bin_Ter_sem_equiv.
+  intros. revert st1 st2. induction c; intros; simpl.
+  - apply H.
+  - apply H0.
+  - apply H1.
+    + intros. apply IHc1.
+    + intros. apply IHc2.
+  - apply H2.
+    + intros. apply IHc1.
+    + intros. apply IHc2.
+  - apply H3.
+    + intros. apply IHc.
+Qed.
+
+Theorem Bin_Step_equiv:
+  sem_equiv (BinRel.ceval) (StepCnt.ceval) (Bin_Ter_sem_equiv).
+Proof.
+  apply (command_equiv__sem_equiv Z BinRel.sem StepCnt.sem
+    Bin_Step_skip_sem_equiv Bin_Step_asgn_sem_equiv
+    Bin_Step_seq_sem_equiv  Bin_Step_if_sem_equiv
+    Bin_Step_loop_sem_equiv).
+Qed.
+
+Theorem Bin_Trace_equiv:
+  sem_equiv (BinRel.ceval) (Trace.ceval) (Bin_Ter_sem_equiv).
+Proof.
+  apply (command_equiv__sem_equiv (list state) BinRel.sem Trace.sem
+    Bin_Trace_skip_sem_equiv Bin_Trace_asgn_sem_equiv
+    Bin_Trace_seq_sem_equiv  Bin_Trace_if_sem_equiv
+    Bin_Trace_loop_sem_equiv).
+Qed.
+
+(* General Theorem for equivalence between two recursively defined semantics *)
+
