README.md
@@ -8,16 +8,50 @@
 
 ## Compilation Order
 
-* Imp3.v
-* ImpExt4.v
-* DenotationalSemantics.v
-* SemEquivLemmas.v
+1. ImpExt4.v
+2. Imp3.v
+3. DenotationalSemantics.v
+4. DenotationalSemEquiv.v
+5. SmallStepSemantics.v
+6. SmallStepSemEquiv.v
 
 ## TODO
 
-- A theorem which can be used to prove the equivalence between two recursively defined semantics
-- A theorem which can be used to prove the equivalence between a recursively defined semantics and a small step semantics
-- Prove the equivalence between three denotational semantics ( *plain binary relation, one with time, one with trace* ) and a small step semantics
+- Prove the theorem which can be used to prove the equivalence between a recursively defined semantics and a small step semantics.
+
+## Done
+
+- Prove a general theorem used to prove an equivalence between two recursively defined semantics.
+- Prove the equivalence between three denotational  semantics.
+- Prove the equivalence between three denotational semantics ( *plain binary relation, one with time, one with trace* ) and a small step semantics.
+
+## Proof Idea
+
+- DenotationalSemantics.v
+
+  We define three denotational program semantics, which are based on the project instruction. However we also make some modification.
+
+  First, we define a general recursively defined denotational semantic, which has five basic commands *(skip, assignment, sequence, if, while)*. A program's semantic is recursively defined on the semantic of the five basic commands.
+
+  Then, we give the definition of three concrete denotational semantics after defining the semantics of five basic commands.
+
+- DenotationalSemEquiv.v
+
+  - Denotation
+
+    We raise and prove a general theorem to prove an equivalence between two recursively defined semantics. We use it to prove the equivalence between three denotational semantics defined in DenotationalSemantics.v.
+
+    First, we define the equivalence of five basic commands between two recursively defined semantics.
+
+    Next, we put forward and prove the general theorem for equivalence between them.
+
+    Then, we prove the equivalence of five basic commands between two concrete semantics defined in DenotationalSemantics.v.
+  
+    At last, we apply the general theorem and finish the proof.
+  
+  - Denotation V.S. Small Step
+  
+    We give a general theorem and use it to prove the equivalence between denotational semantics and small step semantics.
 
 ## Contributor
 
